Title: Some simple recursive functions
Date: 2014-12-17
Category: Python
Authors: Dee Kras

##So how do recursions work?

I hear so much about recursions. They're supposedly in all interview questions.  So here's my attempt at trying to make them easy to understand.

A recursive function is a function that calls itself. I'll throw in a simple example. The factorial.

The factorial of 5 = 5 x 4 x 3 x 2 x 1.  What is happening here:

   - first, 5 is multiplied by 5-1 (in other words 4) = 20
   - then,  that result (20) is multiplied by 4-1 (3)  = 60 
   - then,  that result (60) is multiplied by 3-1 (2) = 120
   - lastly,  that result (120) is multiplied by 2-1 (1) = 120
   - and it's over. We have the result.

There's a repetetive pattern here - the result is multiplied by (the number - 1) `n * (n-1)`. That's where the recursive function comes in.


Here is what the function might look like. I put in lots of print statements so you can see what is happening at each point.  

```python

def factorial(n):
    print "NOW: We're (back) at the beginning of the function. n = {}".format(n)
    if n <= 0:
        return 0
    if n == 1:
        print "--- HIT THE BASE CASE"
        print "NOW: the return is 1."
        print "--- WILL START GOING BACK UP THE LADDER"
        return 1
    else:
        print "   NOW: We're in the 'else statement'. n = {}".format(n)
        result =  n * factorial(n-1)
        print """NOW: The interim result (the previous 'return') is {result_was} and n = {n}.  
              So {result_was} * {n} = {result}.""".format(result_was=result/n, n=n, result=result)
        print "   The NEW interim result (the current 'return') based on this recursion is:  {}.".format(result)
        return result

print factorial(3)

```

###**So what is happening here?**

Let's look at the key line `result =  n * factorial(n-1)`. The number `n` is being multiplied by ... the result of the same function `factorial(n-1)`.  In other words, a loop of the function calling itself.

Let's look at the construct of the rest of the function and we'll come back to that line.   We start off with `if n <= 0:  return 0`. For this function, we don't want to deal with negative numbers or 0. So if the argument is 0 or less, it returns a 0 and that is the end.

Similarly, `if n == 1: return 1`. If the argument of the function is 1, it returns a 1 and that is the end. This line also plays an important role in the overall function. Every recursive function **must have an end to the loop\***, or it will go on in an infinite loop.  So in this case, if the number is equal to 1, it stops the recursion with a `return 1` and then the function finishes up the rest of its work.  (\*This is also referred to as the 'base case' - when a problem can be solved without further recursion.)

Now, let's go back and look at the crux of this function `result =  n * factorial(n-1)`. `n` is to be multiplied by what? a function. (Of course, we can call functions in a function). In this case, it is calling the same function, with a different argument `n - 1`. So `n` will wait until it knows what it should be multiplied with; it will wait for the `return` of that function. 

Here is where it gets interesting. That function will then call itself again. `n` waits for a `return`. And since this is a recursion, there is also a new `n` and that one also waits for a `return`. And the recursive loop goes on  and on - until it hits its 'base case'. And then the `return`s are all in and the `n`s can do their multiplication and be done with it.

In other words, **the recursive loop goes down the ladder and all the `n`s wait for their corresponding `return` - until it hits its 'base case', its absolute bottom.  And then it goes back up the ladder.** The most recent `return` is multiplied to the lowest `n`, the most recent `n`. And the `return` of that multiplication is multiplied to the next lowest `n`. And so on until it reaches the top. And we have our final `return`. That is the result of the function.

###**Let's see that in action. **
Here is the result of the above function - with all the print statements:

```

NOW: We're (back) at the beginning of the function. n = 3
   NOW: We're in the 'else statement'. n = 3
NOW: We're (back) at the beginning of the function. n = 2
   NOW: We're in the 'else statement'. n = 2
NOW: We're (back) at the beginning of the function. n = 1
--- HIT THE BASE CASE
NOW: the return is 1.
--- WILL START GOING BACK UP THE LADDER
NOW: The interim result (the previous 'return') is 1 and n = 2.  So 1 * 2 = 2.
   The NEW interim result (the current 'return') based on this recursion is:  2.
NOW: The interim result (the previous 'return') is 2 and n = 3.  So 2 * 3 = 6.
   The NEW interim result (the current 'return') based on this recursion is:  6.
6

```



Check out the flow of this function using [pythontutor.com](http://pythontutor.com/):  Click on the forward button to see what is happening step by step.
<iframe width="800" height="500" frameborder="0" src="http://pythontutor.com/iframe-embed.html#code=def+factorial(n)%3A%0A++++print+%22NOW%3A+We're+(back)+at+the+beginning+of+the+function.+n+%3D+%7B%7D%22.format(n)%0A++++if+n+%3C%3D+0%3A%0A++++++++return+0%0A++++if+n+%3D%3D+1%3A%0A++++++++print+%22---+HIT+THE+BASE+CASE%22%0A++++++++print+%22NOW%3A+the+return+is+1.%22%0A++++++++print+%22---+WILL+START+GOING+BACK+UP+THE+LADDER%22%0A++++++++return+1%0A++++else%3A%0A++++++++print+%22+++NOW%3A+We're+in+the+'else+statement'.+n+%3D+%7B%7D%22.format(n)%0A++++++++result+%3D++n+*+factorial(n-1)%0A++++++++print+%22%22%22NOW%3A+The+interim+result+(the+previous+'return')+is+%7Bresult_was%7D+and+n+%3D+%7Bn%7D.++%0A++++++++++++++So+%7Bresult_was%7D+*+%7Bn%7D+%3D+%7Bresult%7D.%22%22%22.format(result_was%3Dresult/n,+n%3Dn,+result%3Dresult)%0A++++++++print+%22+++The+NEW+interim+result+(the+current+'return')+based+on+this+recursion+is%3A++%7B%7D.%22.format(result)%0A++++++++return+result%0A%0Aprint+factorial(3)&origin=opt-frontend.js&cumulative=false&heapPrimitives=false&drawParentPointers=false&textReferences=false&showOnlyOutputs=false&py=2&rawInputLstJSON=%5B%5D&curInstr=0&codeDivWidth=350&codeDivHeight=400"> </iframe>

###**So what is happening here - step by step?**


Firstly, we start the function at the beginning and n = 3. Since `n` does not meet the 'if statements', it goes to the 'else statement'.  That's where it finds `result =  n * factorial(n-1)` and it calls the `factorial` function, this time with `n-1` as the argument, as `factorial(2)`. And the 3 waits to find out what it will be multiplied by - what is the result of `factorial(2)`? The loop begins.

Now the `n` is 2. And it too wants to know what to be multiplied by and waits for the results of `factorial(1)`.

And now finally, `n` does equal 1. It has hit 'base case' and returns 1. The `return` = 1. Now it goes 'back up the ladder; now the multiplication can begin! 

The `n` is then multiplied by that previous `return`. So `n` * `return`  = `new return`.  2 * 1 = 2. 

That result, the 2, is the new `return` that the 3 is waiting for.  So again `n` * `return`  = `new return`. 3 * 2 = 6. 

And 6 is our final `return`.

**This is the code without all the extras.**

```python

def factorial(n):
    if n <= 0:
        return 0
    if n == 1:
        return 1
    else:
        return  n * factorial(n-1)

print factorial(3)
```


WOW! That was long. But I hope that is clear. **In very short... The recursion goes down until it hits base case. And then goes up doing the function using the `return` from the previous step.**


---------------------
more: 
http://www.python-course.eu/recursive_functions.php

